finishing lemmas part A + subtle change in untyped value relation

theories/lam/lib/universe/nr_embed_project.v
@@ -38,8 +38,8 @@ Fixpoint ep_pair (τ : nr_type) (dir : direction) : val :=
                                                (inject TCProd ((ep_pair τ1 Embed).{ren (+3)} %1, (ep_pair τ2 Embed).{ren (+3)} %0))))
                    | Project => LamV (LetIn (extract TCProd %0)
                                           (LetIn (Fst %0)
-                                                 (LetIn (extract TCProd %2)
-                                                        (LetIn (Snd %0) ((ep_pair τ1 Project).{ren (+5)} %2 , (ep_pair τ2 Project).{ren (+5)} %0)))))
+                                                 (LetIn (Snd %1)
+                                                        ((ep_pair τ1 Project).{ren (+4)} %1 , (ep_pair τ2 Project).{ren (+4)} %0))))
      end
    | NRTSum τ1 τ2 => match dir with
                   | Embed => LamV (Case %0
@@ -69,7 +69,7 @@ Proof.
     intros dir; try by (destruct dir; (apply inject_typed || apply extract_typed)).
   - (* TProd *) destruct dir.
     + repeat (fold nr_type_type; fold ep_pair; ((rewrite -val_subst_valid; apply context_weakening3) || apply IHτ1 with (dir := Embed) || apply IHτ2 with (dir := Embed) || apply inject_typed || econstructor)).
-    + repeat (fold nr_type_type ep_pair; ((rewrite -val_subst_valid; apply context_weakening5) || apply IHτ1 with (dir := Project) || apply IHτ2 with (dir := Project) || apply (extract_typed TCProd) || econstructor)).
+    + repeat (fold nr_type_type ep_pair; ((rewrite -val_subst_valid; apply context_weakening4) || apply IHτ1 with (dir := Project) || apply IHτ2 with (dir := Project) || apply (extract_typed TCProd) || econstructor)).
   - (* TSum *) destruct dir.
     + repeat ((rewrite -val_subst_valid; apply context_weakening2) || apply IHτ1 with (dir := Embed) || apply IHτ2 with (dir := Embed) || closed_solver || apply inject_typed || econstructor).
     + repeat ((rewrite -val_subst_valid; apply context_weakening2) || apply IHτ1 with (dir := Project) || apply IHτ2 with (dir := Project) || closed_solver || apply (extract_typed TCSum) || econstructor).
